testdata/examples/import/import.gold.v
@@ -2,12 +2,12 @@
 From New.golang Require Import defn.
 Require Export New.code.sync.atomic.
 
+Definition example : go_string := "github.com/goose-lang/goose/testdata/examples/import".
+
 Module example.
 Section code.
 Context `{ffi_syntax}.
 
-
-Definition pkg_name' : go_string := "github.com/goose-lang/goose/testdata/examples/import".
 
 Definition vars' : list (go_string * go_type) := [].
 
@@ -15,17 +15,17 @@ Definition functions' : list (go_string * val) := [].
 
 Definition msets' : list (go_string * (list (go_string * val))) := [].
 
-#[global] Instance info' : PkgInfo pkg_name' :=
+#[global] Instance info' : PkgInfo import.example :=
   {|
     pkg_vars := vars';
     pkg_functions := functions';
     pkg_msets := msets';
-    pkg_imported_pkgs := [atomic.pkg_name'];
+    pkg_imported_pkgs := [atomic];
   |}.
 
 Definition initialize' : val :=
   rec: "initialize'" <> :=
-    globals.package_init pkg_name' (λ: <>,
+    globals.package_init import.example (λ: <>,
       exception_do (do:  atomic.initialize')
       ).
 
